WIP cbor_raw_sort_elem

src/cbor/CBOR.Spec.Raw.Sort.fsti
@@ -1,5 +1,6 @@
 module CBOR.Spec.Raw.Sort
 include CBOR.Spec.Raw.Order
+open CBOR.Spec.Util
 
 noextract [@@noextract_to "krml"]
 val cbor_map_sort
@@ -10,6 +11,7 @@ val cbor_map_sort_correct
   (l: list (raw_data_item & raw_data_item))
 : Lemma
   (ensures (let (res, l') = cbor_map_sort l in
+    List.Tot.length l' == List.Tot.length l /\
     (forall x . List.Tot.memP x l' <==> List.Tot.memP x l) /\
     (List.Tot.no_repeats_p (List.Tot.map fst l') <==> List.Tot.no_repeats_p (List.Tot.map fst l)) /\
     (res == true <==> List.Tot.no_repeats_p (List.Tot.map fst l)) /\
@@ -20,3 +22,55 @@ val cbor_map_sort_correct
   ))
   [SMTPat (cbor_map_sort l)]
 
+let cbor_map_sort_failsafe
+  (l: list (raw_data_item & raw_data_item))
+: Tot (list (raw_data_item & raw_data_item))
+= snd (cbor_map_sort l)
+
+let cbor_map_sort_failsafe_correct
+  (l: list (raw_data_item & raw_data_item))
+: Lemma
+  (let l' = cbor_map_sort_failsafe l in
+    List.Tot.length l' == List.Tot.length l /\
+    (forall x . List.Tot.memP x l' <==> List.Tot.memP x l) /\
+    (List.Tot.no_repeats_p (List.Tot.map fst l) ==> (
+      List.Tot.sorted (map_entry_order deterministically_encoded_cbor_map_key_order _) l' /\
+      List.Tot.no_repeats_p (List.Tot.map fst l')      
+    ))
+  )
+= ()
+
+let cbor_raw_sort_elem
+  (x: raw_data_item)
+: Tot raw_data_item
+= match x with
+  | Map len v -> Map len (cbor_map_sort_failsafe v)
+  | _ -> x
+
+let cbor_raw_sort_elem_ints_optimal
+  (x: raw_data_item)
+: Lemma
+  (requires (raw_data_item_ints_optimal x == true))
+  (ensures (raw_data_item_ints_optimal (cbor_raw_sort_elem x) == true))
+= assert_norm (raw_data_item_ints_optimal == holds_on_raw_data_item raw_data_item_ints_optimal_elem);
+  holds_on_raw_data_item_eq raw_data_item_ints_optimal_elem x;
+  holds_on_raw_data_item_eq raw_data_item_ints_optimal_elem (cbor_raw_sort_elem x);
+  match x with
+  | Map len v ->
+    list_for_all_intro (holds_on_pair raw_data_item_ints_optimal) (cbor_map_sort_failsafe v) (fun x ->
+      List.Tot.for_all_mem (holds_on_pair raw_data_item_ints_optimal) v
+    )
+  | _ -> ()
+
+let cbor_raw_sort_elem_equiv
+  (x: raw_data_item)
+: Lemma
+  (ensures (raw_equiv x (cbor_raw_sort_elem x) == true))
+= raw_equiv_eq x (cbor_raw_sort_elem x);
+  match x with
+  | Map len v ->
+    list_for_all_intro (list_existsb2 (holds_on_pair2 raw_equiv) (cbor_map_sort_failsafe v)) v (fun _ -> assume False);
+    list_for_all_intro (list_existsb2 (holds_on_pair2 raw_equiv) v) (cbor_map_sort_failsafe v) (fun _ -> assume False)    
+  | _ -> raw_equiv_refl x
+
+let cbor_raw_sort = raw_data_item_fmap cbor_raw_sort_elem
